added more structure for input to functions, commented out things that don't build

src/Bitstream.v
@@ -1,17 +1,95 @@
-
+Require Import String.
 Require Import AST.
+Require Import List.
+Require Import Values.
 
-(* any finite bitstream *)
-(* use to state correctness of crypto functions *)
-Inductive finite_bitstream : list val -> Prop :=
-| empty_stream :
-    finite_bitstream nil
-| one_more :
-    forall b l,
-      finite_bitstream l ->
-      finite_bitstream (bit b :: l).
+(* We need easy ways of writing down inputs to cryptol functions *)
+(* They only need base type bit, and structures *)
 
-(* bits with length encoded *)
+(* make some kind of type, convertible to val and strictval *)
+
+Inductive ext_val :=
+| ebit (b : bool)
+| eseq (l : list ext_val)
+| etup (l : list ext_val)
+| erec (f : list (string * ext_val))
+.
+
+Fixpoint to_val (e : ext_val) : val :=
+  let fix go_pair (p : string * ext_val) := 
+      match p with
+      | (s,t) => (s, to_val t)
+      end in
+  let fix go_list_pair (ps : list (string * ext_val)) :=
+      match ps with
+      | nil => nil
+      | p :: ps => (go_pair p) :: (go_list_pair ps)
+      end in
+  match e with
+  | ebit b => bit b
+  | eseq l => thunk_list (map to_val l)
+  | etup l => tuple (map to_val l)
+  | erec f => rec (go_list_pair f)
+  end.
+        
+Fixpoint to_sval (e : ext_val) : strictval :=
+  let fix go_pair (p : string * ext_val) := 
+      match p with
+      | (s,t) => (s, to_sval t)
+      end in
+  let fix go_list_pair (ps : list (string * ext_val)) :=
+      match ps with
+      | nil => nil
+      | p :: ps => (go_pair p) :: (go_list_pair ps)
+      end in
+  match e with
+  | ebit b => sbit b
+  | eseq l => strict_list (map to_sval l)
+  | etup l => stuple (map to_sval l)
+  | erec f => srec (go_list_pair f)
+  end.
+
+Inductive ext_type :=
+| tbit
+| tseq (len : nat) (t : ext_type)
+| ttup (l : list ext_type)
+| trec (l : list (string * ext_type))
+.
+
+Inductive has_type : ext_val -> ext_type -> Prop :=
+| is_bit :
+    forall b,
+      has_type (ebit b) tbit
+| is_seq :
+    forall l t,
+      Forall (fun x => has_type x t) l ->
+      has_type (eseq l) (tseq (length l) t)
+| is_tup :
+    forall l lt,
+      Forall2 has_type l lt ->
+      has_type (etup l) (ttup lt)
+| is_rec :
+    forall l lt,
+      Forall2 has_type (map snd l) lt ->
+      has_type (erec l) (trec (combine (map fst l) lt))
+.
+
+Definition byte : ext_type := tseq 8 tbit.
+Definition bytestream (n : nat) := tseq n byte.
+Definition word : ext_type := tseq 64 tbit.
+
+
+
+Definition n_bits (n : nat) (v : val) : Prop :=
+  exists ev,
+    has_type ev (tseq n tbit) /\ to_val ev = v.
+
+Definition sn_bits (n : nat) (v : strictval) : Prop :=
+  exists ev,
+    has_type ev (tseq n tbit) /\ to_sval ev = v.
+    
+
+(*
 Inductive n_bits : nat -> list val -> Prop :=
 | empty_bits :
     n_bits O nil
@@ -19,7 +97,7 @@ Inductive n_bits : nat -> list val -> Prop :=
     forall n l b,
       n_bits n l ->
       n_bits (S n) (bit b :: l).
-
+*)
 
 Require Import Eager.
 Require Import List.
@@ -40,14 +118,33 @@ Lemma n_bits_eval :
   forall n x ge TE E,
     n_bits n x ->
     exists vs,
-      eager_eval_expr ge TE E (EList (map EValue x)) (strict_list vs) /\ length vs = n.
+      eager_eval_expr ge TE E (EValue x) (strict_list vs) /\ length vs = n.
 Proof.
-  induction 1; intros.
-  eexists. split. econstructor; eauto. simpl. econstructor. reflexivity.
-  destruct IHn_bits. destruct H0.
-  inversion H0.
-  eexists. split. simpl. econstructor. simpl. econstructor. econstructor. econstructor.
-  eauto. reflexivity.
-  simpl. subst.
-  eapply strict_list_injective in H6; eauto. congruence.
+  induction n; intros;
+    unfold n_bits in *;
+    destruct H. destruct H.
+  inversion H. destruct l; simpl in *; try congruence. subst.
+  eexists; split. simpl. econstructor; eauto. instantiate (1 := nil). econstructor; eauto. reflexivity.
+
+  destruct H. inversion H. subst.
+  destruct l; simpl in *; try congruence.
+  inversion H3.
+  subst. inversion H4.
+  subst. inversion H1. subst.
+  edestruct IHn; eauto.
+  eexists; split; eauto.
+  econstructor. eauto.
+  destruct H0.
+
+  
+  eexists; split; eauto.
+  simpl. inversion H0. subst.
+  econstructor. instantiate (1 := (sbit b :: x)).
+  simpl. econstructor; eauto.
+  econstructor. econstructor.
+  simpl. congruence.
+
+  Unshelve. exact tempty.
+  exact sempty.
 Qed.
+
