verif/Induction.v
@@ -1,0 +1,147 @@
+(* This file is an example on how to write normal fixpoints over weird trees *)
+(* These trees come up sometimes when expressing the syntax of programs, especially when representing records *)
+(* This walks you through what seems to be the simplest solution *)
+
+Require Import List.
+Import ListNotations.
+
+
+(* A very common design pattern is for a type to contain lists of itself *)
+(* it could be other things, but it is very commonly lists *)
+
+
+(* This is the simplest example I can think of *)
+Inductive simple_tree :=
+| leaf
+| internal (l : list simple_tree)
+.
+
+
+(* Coq can figure this out *)
+Fixpoint get_leaves (s : simple_tree) : list simple_tree :=
+  match s with
+  | leaf => s :: nil
+  | internal l =>
+    concat (map get_leaves l)
+  end.
+
+
+(* This is particularly common for representing records *)
+(* could also be used to represent a trie *)
+(* B is the type of data at the leaves *)
+(* A is the type of label for internal links *)
+Inductive labeled_tree {A B : Type} :=
+| tleaf (x : B)
+| tinternal (l : list (A * labeled_tree))
+.
+
+(* Now it is hard to write functions over this type *)
+(* Coq doesn't like this: *)
+(* Error: Cannot guess decreasing argument of fix. *)
+(*
+
+Fixpoint map_leaves {A B C : Type} (f : B -> C) (t : @labeled_tree A B) : @labeled_tree A C :=
+  match t with
+  | tleaf x => tleaf (f x)
+  | tinternal l =>
+    let labels := map fst l in
+    let subts := map snd l in
+    let subts' := map (map_leaves f) subts in
+    tinternal (combine labels subts')
+  end.
+
+ *)
+
+(* If we actually want to write this function, we have some fun times ahead of us *)
+
+(* We could try to write a size function which we could use as a decreasing measure *)
+(* But we quickly run into the exact same problem we had before *)
+
+(*
+Fixpoint size {A B : Type} : (t : @labeled_tree A B) : nat :=
+  match t with
+  | tleaf _ => S O
+  | tinternal l => 
+    ???
+  .
+ *)
+
+
+(* If you want, you can define it this way: *)
+Fixpoint map_leaves {A B C : Type} (f : B -> C) (t : @labeled_tree A B) : @labeled_tree A C :=
+  let fix go_pair p :=
+      match p with
+      | (lab,subt) => (lab,map_leaves f subt)
+      end in
+  let fix go_list_pair lp :=
+      match lp with
+      | nil => nil
+      | p :: r => (go_pair p) :: (go_list_pair r)
+      end in
+  match t with
+  | tleaf x => tleaf (f x)
+  | tinternal l => tinternal (go_list_pair l)
+  end.
+
+(* If you want to minimize the number of internal fixes, do more like this *)
+Fixpoint map_leaves' {A B C : Type} (f : B -> C) (t : @labeled_tree A B) : @labeled_tree A C :=
+  let fix go_list_pair lp :=
+      match lp with
+      | nil => nil
+      | (lab,subt) :: r => (lab, map_leaves' f subt) :: (go_list_pair r)
+      end in
+  match t with
+  | tleaf x => tleaf (f x)
+  | tinternal l => tinternal (go_list_pair l)
+  end.
+
+
+(* Now we've defined a bunch of functions, but that's just the
+beginning. Coq is great because we can prove things about our
+programs. Suppose we want to prove things about these functions: *)
+
+(* That requires us to induct over these funny trees *)
+
+(* Suppose we want trees where the labels and the data are nats *)
+(* and we really want all the conatined nats to not be zero *)
+(* but the labels can be anything *)
+(* At this point I have no idea why, but it's a simple example *)
+Inductive nonzero : @labeled_tree nat nat -> Prop :=
+| leaf_nonzero :
+    forall n,
+      n <> O ->
+      nonzero (tleaf n)
+| internal_nonzero :
+    forall l,
+      Forall nonzero (map snd l) ->
+      nonzero (tinternal l)
+.
+
+(* Now, it's easy to write relational properties like the one above, but much harder to prove things about them. *)
+
+(* Suppose we add one to all the leaves *)
+(* This transformation should preserve the nonzero property *)
+Lemma nonzero_succ_preserved :
+  forall t,
+    nonzero t ->
+    nonzero (map_leaves S t).
+Proof.
+  induction t; intros. 
+  - econstructor; eauto.
+
+  - induction l; intros.
+    + inversion H. subst. econstructor; eauto.
+    + inversion H. subst. simpl in H1. inversion H1. subst.
+      assert (nonzero (tinternal l)). econstructor; eauto.
+      specialize (IHl H0).
+      unfold map_leaves. fold (@map_leaves nat nat).
+      econstructor. econstructor.
+
+      destruct a. simpl. simpl in H3.
+      
+      Focus 2.
+      inversion IHl. eassumption.
+      
+      (* However, here we need to know about l0, which means we need better induction *)
+Abort.
+  
